tests/lean/defeq_simp2.lean
@@ -10,7 +10,7 @@ axiom foo3 (n : nat) : n ≥ 0
 example (a b : nat) (H : f a (foo1 a) = f a (foo2 a)) : true :=
 by do
   s ← simp_lemmas.mk_default,
-  get_local `H >>= infer_type >>= s^.rsimplify >>= trace,
+  get_local `H >>= infer_type >>= s^.dsimplify >>= trace,
   constructor
 
 set_option defeq_simplify.canonize_proofs true
@@ -20,7 +20,7 @@ constant x1 : nat -- update the environment to force defeq_canonize cache to be 
 example (a b : nat) (H : f a (foo1 a) = f a (foo2 a)) : true :=
 by do
   s ← simp_lemmas.mk_default,
-  get_local `H >>= infer_type >>= s^.rsimplify >>= trace,
+  get_local `H >>= infer_type >>= s^.dsimplify >>= trace,
   constructor
 
 constant x2 : nat -- update the environment to force defeq_canonize cache to be reset
@@ -28,12 +28,12 @@ constant x2 : nat -- update the environment to force defeq_canonize cache to be 
 example (a b : nat) (H : f a (id (id (id (foo1 a)))) = f a (foo2 a)) : true :=
 by do
   s ← simp_lemmas.mk_default,
-  get_local `H >>= infer_type >>= s^.rsimplify >>= trace,
+  get_local `H >>= infer_type >>= s^.dsimplify >>= trace,
   constructor
 
 -- Example that does not work
 example (a b : nat) (H : (λ x, f x (id (id (id (foo1 x))))) = (λ x, f x (foo2 x))) : true :=
 by do
   s ← simp_lemmas.mk_default,
-  get_local `H >>= infer_type >>= s^.rsimplify >>= trace,
+  get_local `H >>= infer_type >>= s^.dsimplify >>= trace,
   constructor
