tests/lean/defeq_simp3.lean
@@ -12,5 +12,5 @@ set_option pp.all true
 example (a b : nat) (H : (λ x : nat, @add nat nat_has_add2 a x) = (λ x : nat, @add nat (nat_has_add3 x) a b)) : true :=
 by do
   s ← simp_lemmas.mk_default,
-  get_local `H >>= infer_type >>= s^.rsimplify >>= trace,
+  get_local `H >>= infer_type >>= s^.dsimplify >>= trace,
   constructor
