tests/lean/unfold_crash.lean
@@ -5,6 +5,6 @@ example (a b : nat) : a = succ b → a = b + 1 :=
 by do
   H ← intro `H,
   try (unfold_at [`nat.succ] H),
-  unfold [`add], rsimp, unfold [`nat.add],
+  unfold [`add], dsimp, unfold [`nat.add],
   trace_state,
   assumption
